\hspace*{\algorithmicindent} \textbf{Input:} Coefficients $\{ \mu_l \}_{l=0}^{m}$ of the expansion $\sum_{l=0}^{m} \mu_l T_l(s)$ \\
\hspace*{\algorithmicindent} \textbf{Parameter:} Exponent $k$ \\
\hspace*{\algorithmicindent} \textbf{Output:} Coefficients $\{ \nu_l \}_{l=0}^{km}$ such that $\sum_{l=0}^{km} \nu_l T_l(s) = (\sum_{l=0}^{m} \mu_l T_l(s))^k$
\begin{algorithmic}[1]
    \State Define the vector $\widehat{\vct{\mu}}$ as
        \begin{equation}
            (\widehat{\vct{\mu}})_l = \begin{cases} \mu_l &\text{for $l=0, \dots, m$} \\
                                                     0 &\text{for $l=m+1, \dots, km$} \end{cases}
        \end{equation}
    \State Compute $\vct{f} = \DCT(\widehat{\vct{\mu}})$
    \State Let $(\vct{f}^{k})_l = (f_l)^k$ for $l=0, \dots, km$
    \State Compute $\vct{\nu} = \DCT^{-1}(\vct{f}^{k})$
    \State Let $\nu_l = (\vct{\nu})_l$ for $l=0, \dots, km$
\end{algorithmic}
